Lww_inv_b1_b2.fst
@@ -124,7 +124,7 @@ let linearizable_s1_gt0 (lca s1 s2:st) (l':log)
 #pop-options
 
 #push-options "--z3rlimit 100"
-let linearizable_s2_gt01 (lca s1 s2:st) (l':log)
+let linearizable_s2_gt0 (lca s1 s2:st) (l':log)
   : Lemma (requires is_prefix (ops_of lca) (ops_of s1) /\
                     is_prefix (ops_of lca) (ops_of s2) /\
                     Seq.length (ops_of s1) > Seq.length (ops_of lca) /\ Seq.length (ops_of s1) > 0 /\
@@ -149,5 +149,30 @@ let linearizable_s2_gt01 (lca s1 s2:st) (l':log)
   resolve_conflict_prop last1 last2;
   lem_foldl init_st (ops_of s2)
 #pop-options
+
+////////////////////////////////////////////////////////////////
+//// Sequential implementation //////
+
+// the concrete state
+type concrete_st_s = nat
+
+// init state
+let init_st_s = 0
+
+// apply an operation to a state
+let do_s (s:concrete_st_s) (op:log_entry) : concrete_st_s = snd op
+
+//equivalence relation between the concrete states of sequential type and MRDT
+let eq (st_s:concrete_st_s) (st:concrete_st) = st_s = snd st
+
+//initial states are equivalent
+let initial_eq _
+  : Lemma (ensures eq init_st_s init_st) = ()
+
+//equivalence between states of sequential type and MRDT at every operation
+let do_eq (st_s:concrete_st_s) (st:concrete_st) (op:log_entry)
+  : Lemma (requires eq st_s st)
+          (ensures eq (do_s st_s op) (do st op)) 
+  = ()
 
 
