Ew_inv_b1_b2.fst
@@ -1,0 +1,366 @@
+module Ew_inv_b1_b2
+
+open FStar.Seq
+open FStar.Ghost
+
+// the concrete state type
+// It is a pair of counter and boolean representing the flag state
+type concrete_st = nat & bool
+
+//initial state
+let init_st = (0, false)
+
+// operation type
+// (the only operation is Write value, so nat is fine)
+type op_t:eqtype = 
+  |Enable
+  |Disable
+
+// apply an operation to a state
+let do (s:concrete_st) (o:log_entry) : concrete_st = 
+  match snd o with
+  |Enable -> (fst s + 1, true)
+  |Disable -> (fst s, false)
+
+let rec count_en (l:log) : Tot nat (decreases length l) =
+  match length l with
+  |0 -> 0
+  |_ -> match snd (head l) with
+       |Enable -> 1 + count_en (tail l)
+       |_ -> count_en (tail l)
+
+let rec lem_foldl (s:concrete_st) (l:log)
+  : Lemma (ensures (fst (linearized_merge s l) = fst s + count_en l) /\
+                   ((length l > 0 /\ (exists e. mem e l /\ snd e = Enable)) <==> fst (linearized_merge s l) > fst s) /\
+                   ((length l = 0 \/ (length l > 0 /\ (forall e. mem e l ==> snd e <> Enable))) <==> fst (linearized_merge s l) = fst s) /\
+                   (((length l > 0 /\ snd (last l) = Disable) \/
+                   (length l = 0 /\ snd s = false)) <==> snd (linearized_merge s l) = false) /\
+                   (((length l > 0 /\ snd (last l) = Enable) \/
+                   (length l = 0 /\ snd s = true)) <==> snd (linearized_merge s l) = true))
+          (decreases length l)
+  = match length l with
+    |0 -> ()
+    |_ -> lem_foldl (do s (head l)) (tail l)
+
+//conflict resolution
+let resolve_conflict (x y:log_entry) : (l:log{forall e. mem e l <==> e = x \/ e = y}) =
+  if snd x = Enable && snd y = Disable then
+     cons y (cons x empty) else
+       cons x (cons y empty)
+
+#push-options "--z3rlimit 50"
+let resolve_conflict_prop (x y:log_entry)
+  : Lemma (requires fst x <> fst y)
+          (ensures Seq.length (resolve_conflict x y) = 2 /\
+                   ((snd x = Disable /\ snd y = Disable) ==> count_en (resolve_conflict x y) = 0) /\
+                   ((snd x = Enable /\ snd y = Enable) ==> count_en (resolve_conflict x y) = 2) /\
+            (((snd x = Enable /\ snd y = Disable) \/ (snd x = Disable /\ snd y = Enable)) ==> count_en (resolve_conflict x y) = 1) /\
+            (snd x = Enable /\ snd y = Disable <==> last (resolve_conflict x y) = x) /\
+            (snd x <> Enable \/ snd y <> Disable <==> last (resolve_conflict x y) = y) /\
+            (last (resolve_conflict x y) <> x <==> last (resolve_conflict x y) = y) /\
+            (last (resolve_conflict x y) <> y <==> last (resolve_conflict x y) = x) /\
+            (last (resolve_conflict x y) <> x <==> snd x <> Enable \/ snd y <> Disable) /\
+            (last (resolve_conflict x y) <> y <==> snd x = Enable /\ snd y = Disable))
+  = ()
+
+// concrete merge pre-condition
+let concrete_merge_pre lca a b : prop
+  = fst a >= fst lca /\ fst b >= fst lca
+
+val merge_flag : l:concrete_st
+               -> a:concrete_st
+               -> b:concrete_st{concrete_merge_pre l a b}
+               -> Tot (b1:bool {(b1 = true <==> (snd a = true /\ fst a > fst l) \/
+                                             (snd b = true /\ fst b > fst l) \/
+                                             (snd a = true /\ snd b = true) \/ 
+                                             (snd a = true /\ snd b = false /\ fst a > fst l) \/
+                                             (snd b = true /\ snd a = false /\ fst b > fst l)) /\
+                               (b1 = false <==> (snd a = false /\ fst b = fst l) \/
+                                              (snd b = false /\ fst a = fst l) \/
+                                              (snd a = false /\ snd b = false) \/ 
+                                              (snd a = true /\ snd b = false /\ fst a = fst l) \/
+                                              (snd b = true /\ snd a = false /\ fst b = fst l))})
+let merge_flag l a b =
+  let lc = fst l in
+  let ac = fst a in
+  let bc = fst b in
+  let af = snd a in
+  let bf = snd b in
+    if af && bf then true
+      else if not af && not bf then false
+        else if af then ac - lc > 0
+          else bc - lc > 0
+
+// concrete merge operation
+let concrete_merge (lca:concrete_st) (s1:concrete_st) (s2:concrete_st{concrete_merge_pre lca s1 s2}) : concrete_st = 
+  (fst s1 + fst s2 - fst lca, merge_flag lca s1 s2)
+
+#push-options "--z3rlimit 50"
+let merge_prop (lca s1 s2:st)
+  : Lemma (requires is_prefix (ops_of lca) (ops_of s1) /\ 
+                    is_prefix (ops_of lca) (ops_of s2))
+          (ensures concrete_merge_pre (v_of lca) (v_of s1) (v_of s2)) = 
+  lem_foldl init_st (ops_of s1); 
+  lem_foldl init_st (ops_of s2);
+  split_prefix init_st (ops_of lca) (ops_of s1);
+  split_prefix init_st (ops_of lca) (ops_of s2);
+  lem_foldl (v_of lca) (diff (ops_of s1) (ops_of lca));
+  lem_foldl (v_of lca) (diff (ops_of s2) (ops_of lca))
+
+let merge_inv_s1_prop (lca s1 s2:st)
+  : Lemma (requires is_prefix (ops_of lca) (ops_of s1) /\
+                    is_prefix (ops_of lca) (ops_of s2) /\
+                    length (ops_of s1) > length (ops_of lca))
+          (ensures concrete_merge_pre (v_of lca) (v_of (inverse_st s1)) (v_of s2)) =
+  lem_foldl init_st (ops_of s2); 
+  lem_foldl init_st (ops_of (inverse_st s1));
+  lem_inverse (ops_of lca) (ops_of s1);
+  split_prefix init_st (ops_of lca) (ops_of (inverse_st s1));
+  split_prefix init_st (ops_of lca) (ops_of s2);
+  lem_foldl (v_of lca) (diff (ops_of (inverse_st s1)) (ops_of lca));
+  lem_foldl (v_of lca) (diff (ops_of s2) (ops_of lca))
+
+let merge_inv_s2_prop (lca s1 s2:st)
+  : Lemma (requires is_prefix (ops_of lca) (ops_of s1) /\
+                    is_prefix (ops_of lca) (ops_of s2) /\
+                    length (ops_of s2) > length (ops_of lca))
+          (ensures concrete_merge_pre (v_of lca) (v_of s1) (v_of (inverse_st s2))) =
+  lem_foldl init_st (ops_of s1);
+  lem_foldl init_st (ops_of (inverse_st s2));
+  lem_inverse (ops_of lca) (ops_of s2);
+  split_prefix init_st (ops_of lca) (ops_of (inverse_st s2));
+  split_prefix init_st (ops_of lca) (ops_of s1);
+  lem_foldl (v_of lca) (diff (ops_of (inverse_st s2)) (ops_of lca));
+  lem_foldl (v_of lca) (diff (ops_of s1) (ops_of lca))
+
+let linearizable_s1_0 (lca s1 s2:st)
+  : Lemma 
+      (requires concrete_merge_pre (v_of lca) (v_of s1) (v_of s2) /\
+                is_prefix (ops_of lca) (ops_of s1) /\
+                is_prefix (ops_of lca) (ops_of s2) /\
+                ops_of s1 = ops_of lca /\
+                (forall id id1. mem_id id (ops_of lca) /\ mem_id id1 (diff (ops_of s1) (ops_of lca)) ==> lt id id1) /\
+                (forall id id1. mem_id id (ops_of lca) /\ mem_id id1 (diff (ops_of s2) (ops_of lca)) ==> lt id id1) /\
+                (forall id. mem_id id (diff (ops_of s1) (ops_of lca)) ==> not (mem_id id (diff (ops_of s2) (ops_of lca)))))
+      (ensures concrete_merge (v_of lca) (v_of s1) (v_of s2) == 
+               seq_foldl do (v_of lca) (diff (ops_of s2) (ops_of lca))) =
+  lem_foldl init_st (ops_of lca);
+  lem_foldl init_st (ops_of s1);
+  lem_foldl init_st (ops_of s2);
+  split_prefix init_st (ops_of lca) (ops_of s2);
+  lem_foldl (v_of lca) (diff (ops_of s2) (ops_of lca))
+  
+let linearizable_s2_0 (lca s1 s2:st)
+  : Lemma 
+      (requires concrete_merge_pre (v_of lca) (v_of s1) (v_of s2) /\
+                is_prefix (ops_of lca) (ops_of s1) /\
+                is_prefix (ops_of lca) (ops_of s2) /\
+                Seq.length (ops_of s1) > Seq.length (ops_of lca) /\
+                ops_of s2 = ops_of lca /\
+                (forall id id1. mem_id id (ops_of lca) /\ mem_id id1 (diff (ops_of s1) (ops_of lca)) ==> lt id id1) /\
+                (forall id id1. mem_id id (ops_of lca) /\ mem_id id1 (diff (ops_of s2) (ops_of lca)) ==> lt id id1) /\
+                (forall id. mem_id id (diff (ops_of s1) (ops_of lca)) ==> not (mem_id id (diff (ops_of s2) (ops_of lca)))))
+      (ensures concrete_merge (v_of lca) (v_of s1) (v_of s2) == 
+               seq_foldl do (v_of lca) (diff (ops_of s1) (ops_of lca))) =
+  lem_foldl init_st (ops_of lca);
+  lem_foldl init_st (ops_of s1);
+  lem_foldl init_st (ops_of s2);
+  split_prefix init_st (ops_of lca) (ops_of s1);
+  lem_foldl (v_of lca) (diff (ops_of s1) (ops_of lca))
+
+let lem_add (lca s1 s2:nat)
+  : Lemma (ensures s1 - 1 + s2 - lca + 1 = s1 + s2 - lca /\
+                   s1 + s2 - 1 - lca + 1 = s1 + s2 - lca)
+  = ()
+
+#push-options "--z3rlimit 100"
+let linearizable_s1_gt0 (lca s1 s2:st) (l':log)
+  : Lemma (requires is_prefix (ops_of lca) (ops_of s1) /\
+                    is_prefix (ops_of lca) (ops_of s2) /\
+                    Seq.length (ops_of s1) > Seq.length (ops_of lca) /\ Seq.length (ops_of s1) > 0 /\
+                    Seq.length (ops_of s2) > Seq.length (ops_of lca) /\ Seq.length (ops_of s2) > 0 /\
+                    is_prefix (ops_of lca) (ops_of (inverse_st s1)) /\
+                    concrete_merge_pre (v_of lca) (v_of s1) (v_of s2) /\
+                    concrete_merge_pre (v_of lca) (v_of (inverse_st s1)) (v_of s2) /\
+                    interleaving_predicate l' lca (inverse_st s1) s2 /\
+                    (forall id id1. mem_id id (ops_of lca) /\ mem_id id1 (diff (ops_of s1) (ops_of lca)) ==> lt id id1) /\
+                    (forall id id1. mem_id id (ops_of lca) /\ mem_id id1 (diff (ops_of s2) (ops_of lca)) ==> lt id id1) /\
+                    (forall id. mem_id id (diff (ops_of s1) (ops_of lca)) ==> not (mem_id id (diff (ops_of s2) (ops_of lca)))) /\
+                    (let _, last1 = un_snoc (ops_of s1) in
+                     let _, last2 = un_snoc (ops_of s2) in
+                     last (resolve_conflict last1 last2) = last1))
+          (ensures (let _, last1 = un_snoc (ops_of s1) in
+                   concrete_merge (v_of lca) (v_of s1) (v_of s2) ==
+                   do (concrete_merge (v_of lca) (v_of (inverse_st s1)) (v_of s2)) last1)) =
+  let p1, last1 = un_snoc (ops_of s1) in
+  let _, last2 = un_snoc (ops_of s2) in
+  lastop_neq (ops_of lca) (ops_of s1) (ops_of s2);
+  resolve_conflict_prop last1 last2;
+  assert (snd last1 = Enable /\ snd last2 = Disable);
+  inverse_helper init_st p1 last1;
+  assert (fst (v_of (inverse_st s1)) + fst (v_of s2) - fst (v_of lca) =
+          fst (v_of s1) - 1 + fst (v_of s2) - fst (v_of lca));
+  lem_add (fst (v_of lca)) (fst (v_of s1)) (fst (v_of s2));
+  assert ((fst (v_of s1) - 1 + fst (v_of s2) - fst (v_of lca) + 1) =
+          (fst (v_of s1) + fst (v_of s2) - fst (v_of lca)));
+  assert (fst (concrete_merge (v_of lca) (v_of (inverse_st s1)) (v_of s2)) + 1 =
+          fst (concrete_merge (v_of lca) (v_of s1) (v_of s2)));
+  lem_foldl (v_of lca) (diff (ops_of s1) (ops_of lca)); 
+  assert (fst (v_of s1) > fst (v_of lca));
+  assert (merge_flag (v_of lca) (v_of s1) (v_of s2) = true);
+  ()
+
+let linearizable_s2_gt01 (lca s1 s2:st) (l':log)
+  : Lemma (requires is_prefix (ops_of lca) (ops_of s1) /\
+                    is_prefix (ops_of lca) (ops_of s2) /\
+                    Seq.length (ops_of s1) > Seq.length (ops_of lca) /\ Seq.length (ops_of s1) > 0 /\
+                    Seq.length (ops_of s2) > Seq.length (ops_of lca) /\ Seq.length (ops_of s2) > 0 /\
+                    is_prefix (ops_of lca) (ops_of (inverse_st s2)) /\
+                    concrete_merge_pre (v_of lca) (v_of s1) (v_of s2) /\
+                    concrete_merge_pre (v_of lca) (v_of s1) (v_of (inverse_st s2)) /\
+                    interleaving_predicate l' lca s1 (inverse_st s2) /\
+                    (forall id id1. mem_id id (ops_of lca) /\ mem_id id1 (diff (ops_of s1) (ops_of lca)) ==> lt id id1) /\
+                    (forall id id1. mem_id id (ops_of lca) /\ mem_id id1 (diff (ops_of s2) (ops_of lca)) ==> lt id id1) /\
+                    (forall id. mem_id id (diff (ops_of s1) (ops_of lca)) ==> not (mem_id id (diff (ops_of s2) (ops_of lca)))) /\
+                    (let _, last1 = un_snoc (ops_of s1) in
+                     let _, last2 = un_snoc (ops_of s2) in
+                     last (resolve_conflict last1 last2) <> last1 /\
+                     snd last1 = Disable /\ snd last2 = Disable))
+          (ensures (let _, last2 = un_snoc (ops_of s2) in
+                   concrete_merge (v_of lca) (v_of s1) (v_of s2) ==
+                   do (concrete_merge (v_of lca) (v_of s1) (v_of (inverse_st s2))) last2)) = 
+  let _, last1 = un_snoc (ops_of s1) in
+  let p2, last2 = un_snoc (ops_of s2) in
+  lastop_neq (ops_of lca) (ops_of s1) (ops_of s2);
+  resolve_conflict_prop last1 last2;
+  inverse_helper init_st p2 last2;
+  lem_foldl (v_of lca) (diff (ops_of s2) (ops_of lca));
+  lem_foldl init_st (ops_of s1);
+  lem_foldl init_st (ops_of s2)
+
+let linearizable_s2_gt02 (lca s1 s2:st) (l':log)
+  : Lemma (requires is_prefix (ops_of lca) (ops_of s1) /\
+                    is_prefix (ops_of lca) (ops_of s2) /\
+                    Seq.length (ops_of s1) > Seq.length (ops_of lca) /\ Seq.length (ops_of s1) > 0 /\
+                    Seq.length (ops_of s2) > Seq.length (ops_of lca) /\ Seq.length (ops_of s2) > 0 /\
+                    is_prefix (ops_of lca) (ops_of (inverse_st s2)) /\
+                    concrete_merge_pre (v_of lca) (v_of s1) (v_of s2) /\
+                    concrete_merge_pre (v_of lca) (v_of s1) (v_of (inverse_st s2)) /\
+                    interleaving_predicate l' lca s1 (inverse_st s2) /\
+                    (forall id id1. mem_id id (ops_of lca) /\ mem_id id1 (diff (ops_of s1) (ops_of lca)) ==> lt id id1) /\
+                    (forall id id1. mem_id id (ops_of lca) /\ mem_id id1 (diff (ops_of s2) (ops_of lca)) ==> lt id id1) /\
+                    (forall id. mem_id id (diff (ops_of s1) (ops_of lca)) ==> not (mem_id id (diff (ops_of s2) (ops_of lca)))) /\
+                    (let _, last1 = un_snoc (ops_of s1) in
+                     let _, last2 = un_snoc (ops_of s2) in
+                     last (resolve_conflict last1 last2) <> last1 /\
+                     snd last1 = Enable /\ snd last2 = Enable))
+          (ensures (let _, last2 = un_snoc (ops_of s2) in
+                   concrete_merge (v_of lca) (v_of s1) (v_of s2) ==
+                   do (concrete_merge (v_of lca) (v_of s1) (v_of (inverse_st s2))) last2)) = 
+  let _, last1 = un_snoc (ops_of s1) in
+  let p2, last2 = un_snoc (ops_of s2) in
+  lastop_neq (ops_of lca) (ops_of s1) (ops_of s2);
+  resolve_conflict_prop last1 last2;
+  lem_foldl (v_of lca) (diff (ops_of s2) (ops_of lca));
+  inverse_helper init_st p2 last2;
+  assert (fst (v_of s1) + fst (v_of (inverse_st s2)) - fst (v_of lca) =
+          fst (v_of s1) + fst (v_of s2) - 1 - fst (v_of lca));
+  lem_add (fst (v_of lca)) (fst (v_of s1)) (fst (v_of s2));
+  assert ((fst (v_of s1) + fst (v_of s2) - 1 - fst (v_of lca) + 1) =
+          (fst (v_of s1) + fst (v_of s2) - fst (v_of lca)));
+  assert (fst (concrete_merge (v_of lca) (v_of s1) (v_of (inverse_st s2))) + 1 =
+          fst (concrete_merge (v_of lca) (v_of s1) (v_of s2)));
+  lem_foldl init_st (ops_of s1);
+  lem_foldl init_st (ops_of s2)
+#pop-options
+
+#push-options "--z3rlimit 100"
+let linearizable_s2_gt03 (lca s1 s2:st) (l':log)
+  : Lemma (requires is_prefix (ops_of lca) (ops_of s1) /\
+                    is_prefix (ops_of lca) (ops_of s2) /\
+                    Seq.length (ops_of s1) > Seq.length (ops_of lca) /\ Seq.length (ops_of s1) > 0 /\
+                    Seq.length (ops_of s2) > Seq.length (ops_of lca) /\ Seq.length (ops_of s2) > 0 /\
+                    is_prefix (ops_of lca) (ops_of (inverse_st s2)) /\
+                    concrete_merge_pre (v_of lca) (v_of s1) (v_of s2) /\
+                    concrete_merge_pre (v_of lca) (v_of s1) (v_of (inverse_st s2)) /\
+                    interleaving_predicate l' lca s1 (inverse_st s2) /\
+                    (forall id id1. mem_id id (ops_of lca) /\ mem_id id1 (diff (ops_of s1) (ops_of lca)) ==> lt id id1) /\
+                    (forall id id1. mem_id id (ops_of lca) /\ mem_id id1 (diff (ops_of s2) (ops_of lca)) ==> lt id id1) /\
+                    (forall id. mem_id id (diff (ops_of s1) (ops_of lca)) ==> not (mem_id id (diff (ops_of s2) (ops_of lca)))) /\
+                    (let _, last1 = un_snoc (ops_of s1) in
+                     let _, last2 = un_snoc (ops_of s2) in
+                     last (resolve_conflict last1 last2) <> last1 /\
+                     snd last1 = Disable /\ snd last2 = Enable))
+          (ensures (let _, last2 = un_snoc (ops_of s2) in
+                   concrete_merge (v_of lca) (v_of s1) (v_of s2) ==
+                   do (concrete_merge (v_of lca) (v_of s1) (v_of (inverse_st s2))) last2)) = 
+  let _, last1 = un_snoc (ops_of s1) in
+  let p2, last2 = un_snoc (ops_of s2) in
+  lastop_neq (ops_of lca) (ops_of s1) (ops_of s2);
+  resolve_conflict_prop last1 last2;
+  lem_foldl (v_of lca) (diff (ops_of s2) (ops_of lca));
+  inverse_helper init_st p2 last2;
+  assert (fst (v_of s1) + fst (v_of (inverse_st s2)) - fst (v_of lca) =
+          fst (v_of s1) + fst (v_of s2) - 1 - fst (v_of lca));
+  lem_add (fst (v_of lca)) (fst (v_of s1)) (fst (v_of s2));
+  assert ((fst (v_of s1) + fst (v_of s2) - 1 - fst (v_of lca) + 1) =
+          (fst (v_of s1) + fst (v_of s2) - fst (v_of lca)));
+  assert (fst (concrete_merge (v_of lca) (v_of s1) (v_of (inverse_st s2))) + 1 =
+          fst (concrete_merge (v_of lca) (v_of s1) (v_of s2)));
+  assert (fst (v_of s2) > fst (v_of lca));
+  assert (merge_flag (v_of lca) (v_of s1) (v_of s2) = true);
+  ()
+#pop-options
+
+let linearizable_s2_gt0 (lca s1 s2:st) (l':log)
+  : Lemma (requires is_prefix (ops_of lca) (ops_of s1) /\
+                    is_prefix (ops_of lca) (ops_of s2) /\
+                    Seq.length (ops_of s1) > Seq.length (ops_of lca) /\ Seq.length (ops_of s1) > 0 /\
+                    Seq.length (ops_of s2) > Seq.length (ops_of lca) /\ Seq.length (ops_of s2) > 0 /\
+                    is_prefix (ops_of lca) (ops_of (inverse_st s2)) /\
+                    concrete_merge_pre (v_of lca) (v_of s1) (v_of s2) /\
+                    concrete_merge_pre (v_of lca) (v_of s1) (v_of (inverse_st s2)) /\
+                    interleaving_predicate l' lca s1 (inverse_st s2) /\
+                    (forall id id1. mem_id id (ops_of lca) /\ mem_id id1 (diff (ops_of s1) (ops_of lca)) ==> lt id id1) /\
+                    (forall id id1. mem_id id (ops_of lca) /\ mem_id id1 (diff (ops_of s2) (ops_of lca)) ==> lt id id1) /\
+                    (forall id. mem_id id (diff (ops_of s1) (ops_of lca)) ==> not (mem_id id (diff (ops_of s2) (ops_of lca)))) /\
+                    (let _, last1 = un_snoc (ops_of s1) in
+                     let _, last2 = un_snoc (ops_of s2) in
+                     last (resolve_conflict last1 last2) <> last1))
+          (ensures (let _, last2 = un_snoc (ops_of s2) in
+                   concrete_merge (v_of lca) (v_of s1) (v_of s2) ==
+                   do (concrete_merge (v_of lca) (v_of s1) (v_of (inverse_st s2))) last2)) =
+  let _, last1 = un_snoc (ops_of s1) in
+  let _, last2 = un_snoc (ops_of s2) in
+  lastop_neq (ops_of lca) (ops_of s1) (ops_of s2);
+  resolve_conflict_prop last1 last2;
+  match snd last1, snd last2 with
+  |Disable, Disable -> linearizable_s2_gt01 lca s1 s2 l'
+  |Disable, Enable -> linearizable_s2_gt03 lca s1 s2 l'
+  |Enable, Enable -> linearizable_s2_gt02 lca s1 s2 l'
+
+////////////////////////////////////////////////////////////////
+//// Sequential implementation //////
+
+// the concrete state 
+type concrete_st_s = bool
+
+// init state 
+let init_st_s = false
+
+// apply an operation to a state 
+let do_s (s:concrete_st_s) (op:log_entry) : concrete_st_s = 
+  if snd op = Enable then true else false
+
+//equivalence relation between the concrete states of sequential type and MRDT
+let eq (st_s:concrete_st_s) (st:concrete_st) = st_s = snd st
+
+//initial states are equivalent
+let initial_eq _
+  : Lemma (ensures eq init_st_s init_st) = ()
+
+//equivalence between states of sequential type and MRDT at every operation
+let do_eq (st_s:concrete_st_s) (st:concrete_st) (op:log_entry)
+  : Lemma (requires eq st_s st)
+          (ensures eq (do_s st_s op) (do st op)) 
+  = ()
